<?xml version="1.0" encoding="utf-8"?>
<rdf:RDF
   xmlns:dcterms="http://purl.org/dc/terms/"
   xmlns:ns1="http://www.opengis.net/def/metamodel/ogc-na/"
   xmlns:rdf="http://www.w3.org/1999/02/22-rdf-syntax-ns#"
   xmlns:rdfs="http://www.w3.org/2000/01/rdf-schema#"
   xmlns:skos="http://www.w3.org/2004/02/skos/core#"
>
  <rdf:Description rdf:about="http://www.opengis.net/def/rel/iana/1.0/item">
    <rdf:type rdf:resource="http://www.w3.org/2004/02/skos/core#Concept"/>
    <rdfs:comment>Registered with IANA</rdfs:comment>
    <rdfs:label>item</rdfs:label>
    <dcterms:created rdf:datatype="http://www.w3.org/2001/XMLSchema#date">2020-06-10</dcterms:created>
    <ns1:status rdf:resource="http://www.opengis.net/def/status/valid"/>
    <skos:definition xml:lang="en"> The target IRI points to a resource that is a member of the collection represented by the context IRI.</skos:definition>
    <skos:notation rdf:datatype="https://www.iana.org/assignments/link-relations">item</skos:notation>
    <skos:prefLabel xml:lang="en">item</skos:prefLabel>
    <skos:inScheme rdf:resource="http://www.opengis.net/def/rel"/>
  </rdf:Description>
  <rdf:Description rdf:about="http://www.opengis.net/def/rel/ogc/1.0/items">
    <rdf:type rdf:resource="http://www.w3.org/2004/02/skos/core#Concept"/>
    <rdfs:comment>Not yet registered with IANA</rdfs:comment>
    <rdfs:label>items</rdfs:label>
    <dcterms:created rdf:datatype="http://www.w3.org/2001/XMLSchema#date">2020-06-10</dcterms:created>
    <ns1:status rdf:resource="http://www.opengis.net/def/status/proposed"/>
    <skos:definition xml:lang="en"> Refers to a resource that is comprised of members of the collection represented by the link’s context.</skos:definition>
    <skos:notation>items</skos:notation>
    <skos:prefLabel xml:lang="en">items</skos:prefLabel>
    <skos:inScheme rdf:resource="http://www.opengis.net/def/rel"/>
  </rdf:Description>
  <rdf:Description rdf:about="http://www.opengis.net/def/rel/">
    <rdf:type rdf:resource="http://www.w3.org/2004/02/skos/core#Collection"/>
    <rdfs:label>OGC Link Relation Type Register</rdfs:label>
    <skos:definition xml:lang="en">This is a register of link relation types used by OGC standards.</skos:definition>
    <skos:inScheme rdf:resource="http://www.opengis.net/def/rel"/>
    <skos:member rdf:resource="http://www.opengis.net/def/rel/ogc/1.0/exceptions"/>
    <skos:member rdf:resource="http://www.opengis.net/def/rel/ogc/1.0/execute"/>
    <skos:member rdf:resource="http://www.opengis.net/def/rel/ogc/1.0/job-list"/>
    <skos:member rdf:resource="http://www.opengis.net/def/rel/ogc/1.0/processes"/>
    <skos:member rdf:resource="http://www.opengis.net/def/rel/ogc/1.0/results"/>
    <skos:member rdf:resource="http://www.opengis.net/def/rel/ogc/1.0/conformance"/>
    <skos:member rdf:resource="http://www.opengis.net/def/rel/ogc/1.0/data"/>
    <skos:member rdf:resource="http://www.opengis.net/def/rel/ogc/1.0/items"/>
    <skos:member rdf:resource="http://www.opengis.net/def/rel/iana/1.0/service-doc"/>
    <skos:member rdf:resource="http://www.opengis.net/def/rel/iana/1.0/alternate"/>
    <skos:member rdf:resource="http://www.opengis.net/def/rel/iana/1.0/service-desc"/>
    <skos:member rdf:resource="http://www.opengis.net/def/rel/iana/1.0/self"/>
    <skos:member rdf:resource="http://www.opengis.net/def/rel/iana/1.0/collection"/>
    <skos:member rdf:resource="http://www.opengis.net/def/rel/iana/1.0/prev"/>
    <skos:member rdf:resource="http://www.opengis.net/def/rel/iana/1.0/next"/>
    <skos:member rdf:resource="http://www.opengis.net/def/rel/iana/1.0/describedby"/>
    <skos:member rdf:resource="http://www.opengis.net/def/rel/iana/1.0/license"/>
    <skos:member rdf:resource="http://www.opengis.net/def/rel/iana/1.0/item"/>
    <skos:member rdf:resource="http://www.opengis.net/def/rel/ogc/1.0/data-meta"/>
    <skos:prefLabel xml:lang="en">OGC Link Relation Type Register</skos:prefLabel>
  </rdf:Description>
  <rdf:Description rdf:about="http://www.opengis.net/def/rel/ogc/1.0/data">
    <rdf:type rdf:resource="http://www.w3.org/2004/02/skos/core#Concept"/>
    <rdfs:comment>Not yet registered with IANA</rdfs:comment>
    <rdfs:label>data</rdfs:label>
    <dcterms:created rdf:datatype="http://www.w3.org/2001/XMLSchema#date">2020-06-10</dcterms:created>
    <ns1:status rdf:resource="http://www.opengis.net/def/status/proposed"/>
    <skos:definition xml:lang="en"> Indicates that the link’s context is a distribution of a dataset that is an API and refers to the root resource of the dataset in the API.</skos:definition>
    <skos:notation>data</skos:notation>
    <skos:prefLabel xml:lang="en">data</skos:prefLabel>
    <skos:inScheme rdf:resource="http://www.opengis.net/def/rel"/>
  </rdf:Description>
  <rdf:Description rdf:about="http://www.opengis.net/def/rel/ogc/1.0/execute">
    <rdf:type rdf:resource="http://www.w3.org/2004/02/skos/core#Concept"/>
    <rdfs:comment>Not yet registered with IANA</rdfs:comment>
    <rdfs:label>execute</rdfs:label>
    <dcterms:created rdf:datatype="http://www.w3.org/2001/XMLSchema#date">2020-06-10</dcterms:created>
    <ns1:status rdf:resource="http://www.opengis.net/def/status/proposed"/>
    <skos:definition xml:lang="en">The target URI points to the execution endpoint of the server.</skos:definition>
    <skos:notation>execute</skos:notation>
    <skos:prefLabel xml:lang="en">execute</skos:prefLabel>
    <skos:inScheme rdf:resource="http://www.opengis.net/def/rel"/>
  </rdf:Description>
  <rdf:Description rdf:about="http://www.opengis.net/def/rel/ogc/1.0/conformance">
    <rdf:type rdf:resource="http://www.w3.org/2004/02/skos/core#Concept"/>
    <rdfs:comment>Not yet registered with IANA</rdfs:comment>
    <rdfs:label>conformance</rdfs:label>
    <dcterms:created rdf:datatype="http://www.w3.org/2001/XMLSchema#date">2020-06-10</dcterms:created>
    <ns1:status rdf:resource="http://www.opengis.net/def/status/proposed"/>
    <skos:definition xml:lang="en"> Refers to a resource that identifies the specifications that the link’s context conforms to.</skos:definition>
    <skos:notation>conformance</skos:notation>
    <skos:prefLabel xml:lang="en">conformance</skos:prefLabel>
    <skos:inScheme rdf:resource="http://www.opengis.net/def/rel"/>
  </rdf:Description>
  <rdf:Description rdf:about="http://www.opengis.net/def/rel/iana/1.0/describedby">
    <rdf:type rdf:resource="http://www.w3.org/2004/02/skos/core#Concept"/>
    <rdfs:comment>Registered with IANA</rdfs:comment>
    <rdfs:label>describedby</rdfs:label>
    <dcterms:created rdf:datatype="http://www.w3.org/2001/XMLSchema#date">2020-06-10</dcterms:created>
    <ns1:status rdf:resource="http://www.opengis.net/def/status/valid"/>
    <skos:definition xml:lang="en"> Refers to a resource providing information about the link’s context.</skos:definition>
    <skos:notation rdf:datatype="https://www.iana.org/assignments/link-relations">describedby</skos:notation>
    <skos:prefLabel xml:lang="en">describedby</skos:prefLabel>
    <skos:inScheme rdf:resource="http://www.opengis.net/def/rel"/>
  </rdf:Description>
  <rdf:Description rdf:about="http://www.opengis.net/def/rel/iana/1.0/service-desc">
    <rdf:type rdf:resource="http://www.w3.org/2004/02/skos/core#Concept"/>
    <rdfs:comment>Registered with IANA</rdfs:comment>
    <rdfs:label>service-desc</rdfs:label>
    <dcterms:created rdf:datatype="http://www.w3.org/2001/XMLSchema#date">2020-06-10</dcterms:created>
    <ns1:status rdf:resource="http://www.opengis.net/def/status/valid"/>
    <skos:definition xml:lang="en"> Identifies service description for the context that is primarily intended for consumption by machines. API definitions are considered service descriptions.</skos:definition>
    <skos:notation rdf:datatype="https://www.iana.org/assignments/link-relations">service-desc</skos:notation>
    <skos:prefLabel xml:lang="en">service-desc</skos:prefLabel>
    <skos:inScheme rdf:resource="http://www.opengis.net/def/rel"/>
  </rdf:Description>
  <rdf:Description rdf:about="http://www.opengis.net/def/rel/ogc/1.0/results">
    <rdf:type rdf:resource="http://www.w3.org/2004/02/skos/core#Concept"/>
    <rdfs:comment>Not yet registered with IANA</rdfs:comment>
    <rdfs:label>results</rdfs:label>
    <dcterms:created rdf:datatype="http://www.w3.org/2001/XMLSchema#date">2020-06-10</dcterms:created>
    <ns1:status rdf:resource="http://www.opengis.net/def/status/proposed"/>
    <skos:definition xml:lang="en">The target URI points to the results of a job.</skos:definition>
    <skos:notation>results</skos:notation>
    <skos:prefLabel xml:lang="en">results</skos:prefLabel>
    <skos:inScheme rdf:resource="http://www.opengis.net/def/rel"/>
  </rdf:Description>
  <rdf:Description rdf:about="http://www.opengis.net/def/rel/ogc/1.0/processes">
    <rdf:type rdf:resource="http://www.w3.org/2004/02/skos/core#Concept"/>
    <rdfs:comment>Not yet registered with IANA</rdfs:comment>
    <rdfs:label>processes</rdfs:label>
    <dcterms:created rdf:datatype="http://www.w3.org/2001/XMLSchema#date">2020-06-10</dcterms:created>
    <ns1:status rdf:resource="http://www.opengis.net/def/status/proposed"/>
    <skos:definition xml:lang="en">The target URI points to the list of processes the API offers.</skos:definition>
    <skos:notation>processes</skos:notation>
    <skos:prefLabel xml:lang="en">processes</skos:prefLabel>
    <skos:inScheme rdf:resource="http://www.opengis.net/def/rel"/>
  </rdf:Description>
  <rdf:Description rdf:about="http://www.opengis.net/def/rel/iana/1.0/alternate">
    <rdf:type rdf:resource="http://www.w3.org/2004/02/skos/core#Concept"/>
    <rdfs:comment>Registered with IANA</rdfs:comment>
    <rdfs:label>alternate</rdfs:label>
    <dcterms:created rdf:datatype="http://www.w3.org/2001/XMLSchema#date">2020-06-10</dcterms:created>
    <ns1:status rdf:resource="http://www.opengis.net/def/status/valid"/>
    <skos:definition xml:lang="en"> Refers to a substitute for this context.</skos:definition>
    <skos:notation rdf:datatype="https://www.iana.org/assignments/link-relations">alternate</skos:notation>
    <skos:prefLabel xml:lang="en">alternate</skos:prefLabel>
    <skos:inScheme rdf:resource="http://www.opengis.net/def/rel"/>
  </rdf:Description>
  <rdf:Description rdf:about="http://www.opengis.net/def/rel">
    <rdf:type rdf:resource="http://www.w3.org/2004/02/skos/core#ConceptScheme"/>
    <rdfs:label>OGC Link Relation Type Register</rdfs:label>
    <ns1:collectionView rdf:resource="http://www.opengis.net/def/rel/"/>
    <skos:definition xml:lang="en">This is a register of link relation types used by OGC standards. </skos:definition>
    <skos:prefLabel xml:lang="en">OGC Link Relation Type Register</skos:prefLabel>
    <dcterms:source rdf:resource="http://www.opengis.net/def/entities/bodies/ogcna"/>
  </rdf:Description>
  <rdf:Description rdf:about="http://www.opengis.net/def/rel/iana/1.0/service-doc">
    <rdf:type rdf:resource="http://www.w3.org/2004/02/skos/core#Concept"/>
    <rdfs:comment>Registered with IANA</rdfs:comment>
    <rdfs:label>service-doc</rdfs:label>
    <dcterms:created rdf:datatype="http://www.w3.org/2001/XMLSchema#date">2020-06-10</dcterms:created>
    <ns1:status rdf:resource="http://www.opengis.net/def/status/valid"/>
    <skos:definition xml:lang="en"> Identifies service documentation for the context that is primarily intended for human consumption.</skos:definition>
    <skos:notation rdf:datatype="https://www.iana.org/assignments/link-relations">service-doc</skos:notation>
    <skos:prefLabel xml:lang="en">service-doc</skos:prefLabel>
    <skos:inScheme rdf:resource="http://www.opengis.net/def/rel"/>
  </rdf:Description>
  <rdf:Description rdf:about="http://www.opengis.net/def/rel/iana/1.0/prev">
    <rdf:type rdf:resource="http://www.w3.org/2004/02/skos/core#Concept"/>
    <rdfs:comment>Registered with IANA</rdfs:comment>
    <rdfs:label>prev</rdfs:label>
    <dcterms:created rdf:datatype="http://www.w3.org/2001/XMLSchema#date">2020-06-10</dcterms:created>
    <ns1:status rdf:resource="http://www.opengis.net/def/status/valid"/>
    <skos:definition xml:lang="en"> Indicates that the link’s context is a part of a series, and that the previous in the series is the link target. This relation is only used in examples.</skos:definition>
    <skos:notation rdf:datatype="https://www.iana.org/assignments/link-relations">prev</skos:notation>
    <skos:prefLabel xml:lang="en">prev</skos:prefLabel>
    <skos:inScheme rdf:resource="http://www.opengis.net/def/rel"/>
  </rdf:Description>
  <rdf:Description rdf:about="http://www.opengis.net/def/rel/iana/1.0/self">
    <rdf:type rdf:resource="http://www.w3.org/2004/02/skos/core#Concept"/>
    <rdfs:comment>Registered with IANA</rdfs:comment>
    <rdfs:label>self</rdfs:label>
    <dcterms:created rdf:datatype="http://www.w3.org/2001/XMLSchema#date">2020-06-10</dcterms:created>
    <ns1:status rdf:resource="http://www.opengis.net/def/status/valid"/>
    <skos:definition xml:lang="en"> Conveys an identifier for the link’s context.</skos:definition>
    <skos:notation rdf:datatype="https://www.iana.org/assignments/link-relations">self</skos:notation>
    <skos:prefLabel xml:lang="en">self</skos:prefLabel>
    <skos:inScheme rdf:resource="http://www.opengis.net/def/rel"/>
  </rdf:Description>
  <rdf:Description rdf:about="http://www.opengis.net/def/rel/ogc/1.0/exceptions">
    <rdf:type rdf:resource="http://www.w3.org/2004/02/skos/core#Concept"/>
    <rdfs:comment>Not yet registered with IANA</rdfs:comment>
    <rdfs:label>exceptions</rdfs:label>
    <dcterms:created rdf:datatype="http://www.w3.org/2001/XMLSchema#date">2020-06-10</dcterms:created>
    <ns1:status rdf:resource="http://www.opengis.net/def/status/proposed"/>
    <skos:definition xml:lang="en">The target URI points to exceptions of a failed process.</skos:definition>
    <skos:notation>exceptions</skos:notation>
    <skos:prefLabel xml:lang="en">exceptions</skos:prefLabel>
    <skos:inScheme rdf:resource="http://www.opengis.net/def/rel"/>
  </rdf:Description>
  <rdf:Description rdf:about="http://www.opengis.net/def/rel/ogc/1.0/job-list">
    <rdf:type rdf:resource="http://www.w3.org/2004/02/skos/core#Concept"/>
    <rdfs:comment>Not yet registered with IANA</rdfs:comment>
    <rdfs:label>job-list</rdfs:label>
    <dcterms:created rdf:datatype="http://www.w3.org/2001/XMLSchema#date">2020-06-10</dcterms:created>
    <ns1:status rdf:resource="http://www.opengis.net/def/status/proposed"/>
    <skos:definition xml:lang="en">The target URI points to the list of jobs.</skos:definition>
    <skos:notation>job-list</skos:notation>
    <skos:prefLabel xml:lang="en">job-list</skos:prefLabel>
    <skos:inScheme rdf:resource="http://www.opengis.net/def/rel"/>
  </rdf:Description>
  <rdf:Description rdf:about="http://www.opengis.net/def/rel/iana/1.0/next">
    <rdf:type rdf:resource="http://www.w3.org/2004/02/skos/core#Concept"/>
    <rdfs:comment>Registered with IANA</rdfs:comment>
    <rdfs:label>next</rdfs:label>
    <dcterms:created rdf:datatype="http://www.w3.org/2001/XMLSchema#date">2020-06-10</dcterms:created>
    <ns1:status rdf:resource="http://www.opengis.net/def/status/valid"/>
    <skos:definition xml:lang="en"> Indicates that the link’s context is a part of a series, and that the next in the series is the link target.</skos:definition>
    <skos:notation rdf:datatype="https://www.iana.org/assignments/link-relations">next</skos:notation>
    <skos:prefLabel xml:lang="en">next</skos:prefLabel>
    <skos:inScheme rdf:resource="http://www.opengis.net/def/rel"/>
  </rdf:Description>
  <rdf:Description rdf:about="http://www.opengis.net/def/rel/iana/1.0/license">
    <rdf:type rdf:resource="http://www.w3.org/2004/02/skos/core#Concept"/>
    <rdfs:comment>Registered with IANA</rdfs:comment>
    <rdfs:label>license</rdfs:label>
    <dcterms:created rdf:datatype="http://www.w3.org/2001/XMLSchema#date">2020-06-10</dcterms:created>
    <ns1:status rdf:resource="http://www.opengis.net/def/status/valid"/>
    <skos:definition xml:lang="en"> Refers to a license associated with this context.</skos:definition>
    <skos:notation rdf:datatype="https://www.iana.org/assignments/link-relations">license</skos:notation>
    <skos:prefLabel xml:lang="en">license</skos:prefLabel>
    <skos:inScheme rdf:resource="http://www.opengis.net/def/rel"/>
  </rdf:Description>
  <rdf:Description rdf:about="http://www.opengis.net/def/rel/ogc/1.0/data-meta">
    <rdf:type rdf:resource="http://www.w3.org/2004/02/skos/core#Concept"/>
    <rdfs:comment>Not yet registered with IANA</rdfs:comment>
    <rdfs:label>data-meta</rdfs:label>
    <dcterms:created rdf:datatype="http://www.w3.org/2001/XMLSchema#date">2021-04-28</dcterms:created>
    <ns1:status rdf:resource="http://www.opengis.net/def/status/proposed"/>
    <skos:definition xml:lang="en">Identifies general metadata for the context (dataset or collection) that is primarily intended for consumption by machines.</skos:definition>
    <skos:notation>data-meta</skos:notation>
    <skos:prefLabel xml:lang="en">data-meta</skos:prefLabel>
    <skos:inScheme rdf:resource="http://www.opengis.net/def/rel"/>
  </rdf:Description>
  <rdf:Description rdf:about="http://www.opengis.net/def/rel/iana/1.0/collection">
    <rdf:type rdf:resource="http://www.w3.org/2004/02/skos/core#Concept"/>
    <rdfs:comment>Registered with IANA</rdfs:comment>
    <rdfs:label>collection</rdfs:label>
    <dcterms:created rdf:datatype="http://www.w3.org/2001/XMLSchema#date">2020-06-10</dcterms:created>
    <ns1:status rdf:resource="http://www.opengis.net/def/status/valid"/>
    <skos:definition xml:lang="en"> The target IRI points to a resource which represents the collection resource for the context IRI.</skos:definition>
    <skos:notation rdf:datatype="https://www.iana.org/assignments/link-relations">collection</skos:notation>
    <skos:prefLabel xml:lang="en">collection</skos:prefLabel>
    <skos:inScheme rdf:resource="http://www.opengis.net/def/rel"/>
  </rdf:Description>
  <rdf:Description rdf:about="http://www.opengis.net/def/register/">
    <skos:member rdf:resource="http://www.opengis.net/def/rel/"/>
  </rdf:Description>
  <rdf:Description rdf:about="http://www.opengis.net/def/entities/bodies/ogcna">
    <rdf:type rdf:resource="http://www.w3.org/2004/02/skos/core#Concept"/>
  </rdf:Description>
</rdf:RDF>
