@prefix dcterms: <http://purl.org/dc/terms/> .
@prefix ns1: <http://www.opengis.net/def/metamodel/ogc-na/> .
@prefix rdfs: <http://www.w3.org/2000/01/rdf-schema#> .
@prefix skos: <http://www.w3.org/2004/02/skos/core#> .
@prefix xsd: <http://www.w3.org/2001/XMLSchema#> .

<http://www.opengis.net/def/register/> skos:member <http://www.opengis.net/def/wkss/> .

<http://www.opengis.net/def/wkss> a skos:ConceptScheme ;
    rdfs:label "Well-Known Scale Sets (WKSS) Register" ;
    dcterms:created "2020-10-04"^^xsd:date ;
    dcterms:source <http://www.opengis.net/def/entities/bodies/ogcna> ;
    ns1:collectionView <http://www.opengis.net/def/wkss/> ;
    skos:definition "The Well-Known Scale Sets(WKSS) concept was introduced in the Web Map Tile Service (WMTS) standard (OGC 07-057r7) to improve interoperability and further described in the 2D Tile Matrix Set standard (OGC 17-083r2)."@en ;
    skos:prefLabel "Well-Known Scale Sets (WKSS) Register"@en .

<http://www.opengis.net/def/wkss/OGC/1.0/GlobalCRS84Pixel> a skos:Concept ;
    rdfs:label "GlobalCRS84Pixel" ;
    dcterms:created "2020-10-04"^^xsd:date ;
    ns1:status <http://www.opengis.net/def/status/valid> ;
    rdfs:seeAlso <http://docs.opengeospatial.org/is/17-083r2/17-083r2.html#58> ;
    skos:definition "GlobalCRS84Pixel well-known scale set definition"@en ;
    skos:inScheme <http://www.opengis.net/def/wkss/OGC> ;
    skos:prefLabel "GlobalCRS84Pixel"@en .

<http://www.opengis.net/def/wkss/OGC/1.0/GlobalCRS84Scale> a skos:Concept ;
    rdfs:label "GlobalCRS84Scale" ;
    dcterms:created "2020-10-04"^^xsd:date ;
    ns1:status <http://www.opengis.net/def/status/valid> ;
    rdfs:seeAlso <http://docs.opengeospatial.org/is/17-083r2/17-083r2.html#57> ;
    skos:definition "GlobalCRS84Scale well-known scale set definition"@en ;
    skos:inScheme <http://www.opengis.net/def/wkss/OGC> ;
    skos:prefLabel "GlobalCRS84Scale"@en .

<http://www.opengis.net/def/wkss/OGC/1.0/GoogleCRS84Quad> a skos:Concept ;
    rdfs:label "GoogleCRS84Quad" ;
    dcterms:created "2020-10-04"^^xsd:date ;
    ns1:status <http://www.opengis.net/def/status/valid> ;
    rdfs:seeAlso <http://docs.opengeospatial.org/is/17-083r2/17-083r2.html#59> ;
    skos:definition "GoogleCRS84Quad well-known scale set definition"@en ;
    skos:inScheme <http://www.opengis.net/def/wkss/OGC> ;
    skos:prefLabel "GoogleCRS84Quad"@en .

<http://www.opengis.net/def/wkss/OGC/1.0/GoogleMapsCompatible> a skos:Concept ;
    rdfs:label "GoogleMapsCompatible" ;
    dcterms:created "2021-11-30"^^xsd:date ;
    ns1:status <http://www.opengis.net/def/status/valid> ;
    rdfs:seeAlso <http://docs.opengeospatial.org/is/17-083r2/17-083r2.html> ;
    skos:definition "GoogleMapsCompatible well-known scale set definition"@en ;
    skos:inScheme <http://www.opengis.net/def/wkss/OGC> ;
    skos:prefLabel "GoogleMapsCompatible"@en .

<http://www.opengis.net/def/wkss/OGC/1.0/WorldMercatorWGS84> a skos:Concept ;
    rdfs:label "WorldMercatorWGS84" ;
    dcterms:created "2020-10-04"^^xsd:date ;
    ns1:status <http://www.opengis.net/def/status/valid> ;
    rdfs:seeAlso <http://docs.opengeospatial.org/is/17-083r2/17-083r2.html#60> ;
    skos:definition "WorldMercatorWGS84 well-known scale set definition"@en ;
    skos:inScheme <http://www.opengis.net/def/wkss/OGC> ;
    skos:prefLabel "WorldMercatorWGS84"@en .

<http://www.opengis.net/def/entities/bodies/ogcna> a skos:Concept .

<http://www.opengis.net/def/wkss/> a skos:Collection ;
    rdfs:label "Well-Known Scale Sets (WKSS) Register" ;
    dcterms:created "2020-10-04"^^xsd:date ;
    skos:definition "The Well-Known Scale Sets(WKSS) concept was introduced in the Web Map Tile Service (WMTS) standard (OGC 07-057r7) to improve interoperability and further described in the 2D Tile Matrix Set standard (OGC 17-083r2)."@en ;
    skos:inScheme <http://www.opengis.net/def/wkss> ;
    skos:member <http://www.opengis.net/def/wkss/OGC/> ;
    skos:prefLabel "Well-Known Scale Sets (WKSS)"@en .

<http://www.opengis.net/def/wkss/OGC/> a skos:Collection ;
    rdfs:label "OGC Well-Known Scale Sets (WKSS)" ;
    dcterms:created "2020-10-04"^^xsd:date ;
    skos:definition "The Well-Known Scale Sets(WKSS) concept was introduced in the Web Map Tile Service (WMTS) standard (OGC 07-057r7) to improve interoperability and further described in the 2D Tile Matrix Set standard (OGC 17-083r2)."@en ;
    skos:inScheme <http://www.opengis.net/def/wkss/OGC> ;
    skos:member <http://www.opengis.net/def/wkss/OGC/1.0/GlobalCRS84Pixel>,
        <http://www.opengis.net/def/wkss/OGC/1.0/GlobalCRS84Scale>,
        <http://www.opengis.net/def/wkss/OGC/1.0/GoogleCRS84Quad>,
        <http://www.opengis.net/def/wkss/OGC/1.0/GoogleMapsCompatible>,
        <http://www.opengis.net/def/wkss/OGC/1.0/WorldMercatorWGS84> ;
    skos:prefLabel "OGC Well-Known Scale Sets (WKSS)"@en .

<http://www.opengis.net/def/wkss/OGC> a skos:ConceptScheme ;
    rdfs:label "OGC Well-Known Scale Sets (WKSS)" ;
    dcterms:created "2020-10-04"^^xsd:date ;
    dcterms:source <http://www.opengis.net/def/entities/bodies/ogcna> ;
    ns1:collectionView <http://www.opengis.net/def/wkss/OGC/> ;
    skos:definition "The Well-Known Scale Sets(WKSS) concept was introduced in the Web Map Tile Service (WMTS) standard (OGC 07-057r7) to improve interoperability and further described in the 2D Tile Matrix Set standard (OGC 17-083r2)."@en ;
    skos:prefLabel "OGC Well-Known Scale Sets (WKSS)"@en .

